\begin{figure}[H]
    \def\x{1cm}
    \def\y{0.7cm}
    \centering
    \begin{tikzpicture}[every node/.style={scale=0.7}]
        \node[anchor=center](root){};
        \node[on grid, left=       2*\x of root   ](13){$\{a, \neg a\}$};
        \node[on grid, right=      2*\x of root   ](57){$\{b, \neg b\}$};
        \node[on grid, below left= \y and \x of 13](23){$\{a \vee \neg a, \neg a\}$};
        \node[on grid, below right=\y and \x of 13](12){$\{a, a \vee \neg a\}$};
        \node[on grid, below left= \y and \x of 57](67){$\{b \vee \neg b, \neg b\}$};
        \node[on grid, below right=\y and \x of 57](56){$\{b, b \vee \neg b\}$};
        \node[on grid, below right=\y and \x of 23](2){$\{a \vee \neg a\}$};
        \node[on grid, below right=\y and \x of 67](6){$\{b \vee \neg b\}$};
        \coordinate[on grid, below right=0.5*\y and 2*\x of 2](4c){};
        \node[on grid, below=0.5*\y of 4c](4){$\{(a \vee \neg a) \wedge (b \vee \neg b)\}$};

        \draw[-arr] (13) to (23);
        \draw[-arr] (13) to (12);
        \draw[-arr] (57) to (67);
        \draw[-arr] (57) to (56);
        \draw[-arr] (23) to (2);
        \draw[-arr] (12) to (2);
        \draw[-arr] (67) to (6);
        \draw[-arr] (56) to (6);
        \draw[-] (2) to (4c) to (6);
        \draw[-arr] (4c) to (4);
    \end{tikzpicture}
\end{figure}
